dm4good/GuardedPDM.v
@@ -8,12 +8,12 @@ Set Printing Projections.
 Set Universe Polymorphism.
 Unset Universe Minimization ToSet.
 
-Class LeafPred (M : Monad) :=
+Class LeafPred (M : Type → Type) :=
   leaf : ∀ A, A → M A → Prop.
 
 Notation "x ∈ c" := (leaf _ x c) (at level 80).
 
-Class Leafine (M : Monad) (hleaf : LeafPred M) :=
+Class Leafine M (hleaf : LeafPred M) :=
   leafine : ∀ A (c : M A), M { x : A | x ∈ c }.
 
 Arguments leafine {_ _ _} [_].
@@ -22,17 +22,15 @@ Section Guarded.
 
   (* Computation monad *)
 
-  Context {M : Monad}.
+  Context {M} `{Monad M}.
 
   (* Specification monad *)
 
-  Context {W : Monad} {Word : Order W} (hmono : MonoSpec W Word).
-
-  Existing Instance trans.
+  Context {W} `{Monad W} {Word : Order W} (hmono : MonoSpec W).
 
   (* Effect observation *)
 
-  Context {θ : observation M W} (hlax : LaxMorphism Word θ).
+  Context {θ : observation M W} (hlax : LaxMorphism θ).
 
   Arguments θ [_].
 
@@ -41,23 +39,24 @@ Section Guarded.
   Context (leafpred : LeafPred M) (hleaf : Leafine M leafpred).
 
   (* We first build a new computation monad with req *)
-  Definition Mᴳ : ReqMonad.
+
+  Definition Mᴳ A := G (M A).
+
+  #[refine] Instance Monad_Mᴳ : Monad Mᴳ := {|
+    ret A x := ret (M := G) (ret x)
+  |}.
   Proof.
-    simple refine {|
-      Mq := {|
-        Mo A := G (M A) ;
-        ret A x := G.(ret) (M.(ret) x)
-      |} ;
-      req p := G.(bind) (G.(req) p) (λ h, G.(ret) (M.(ret) h))
-    |}.
-    (* bind *)
     hnf. intros A B c f.
     exists (∃ (h : c.π1), ∀ x, x ∈ c.π2 h → (f x).π1). intro h.
-    simple refine (M.(bind) (leafine (c.π2 _)) (λ x, (f (val x)).π2 _)).
+    simple refine (bind (leafine (c.π2 _)) (λ x, (f (val x)).π2 _)).
     - apply h.
     - destruct h as [hp h]. destruct x as [x hx]. apply h.
       apply hx.
   Defined.
+
+  Instance ReqMonad_Mᴳ : ReqMonad Mᴳ := {|
+    req p := bind (req p) (λ h, ret (M := G) (ret (M := M) h))
+  |}.
 
   (* Now we extend the spec monad with req, we do this using a liftᵂ *)
   (* TODO: Should it generally be built this way? *)
@@ -66,18 +65,17 @@ Section Guarded.
 
   Arguments liftᵂ [_].
 
-  Definition Wᴳ : ReqMonad := {|
-    Mq := W ;
-    req p := liftᵂ (pure_wp_reqmon.(req) p)
+  Instance ReqMonad_W : ReqMonad W := {|
+    req p := liftᵂ (req p)
   |}.
 
   (* New effect observation *)
 
-  Definition θᴳ : observation Mᴳ Wᴳ :=
-    λ A c, Wᴳ.(bind) (Wᴳ.(req) c.π1) (λ h, θ (c.π2 h)).
+  Definition θᴳ : observation Mᴳ W :=
+    λ A c, bind (req c.π1) (λ h, θ (c.π2 h)).
 
   (* We now extend the effect observation *)
-  Instance hreqlax : @ReqLaxMorphism Mᴳ Wᴳ Word θᴳ.
+  (* Instance hreqlax : ReqLaxMorphism Word θᴳ.
   Proof.
     constructor. 1: constructor.
     - intros A x.
@@ -95,19 +93,22 @@ Section Guarded.
       unfold θᴳ. cbn - [pure_wp_reqmon].
       (* Not even clear it works *)
       admit.
-  Abort.
+  Abort. *)
 
   (* Until we find the proper assumptions, we will assume it *)
-  Context (hreqlax : @ReqLaxMorphism Mᴳ Wᴳ Word θᴳ).
+  Context (θᴳ_lax : LaxMorphism θᴳ) (θᴳ_reqlax : ReqLaxMorphism Word θᴳ).
 
   (* Partial Dijkstra monad *)
 
-  Definition D : DijkstraMonad Word :=
-    PDM.D (M := Mᴳ) (W := Wᴳ) hmono hreqlax.
+  Definition D A w :=
+    PDM.D (θ := θᴳ) A w.
+
+  Instance DijkstraMonad_D : DijkstraMonad D :=
+    PDM.DijkstraMonad_D hmono θᴳ_lax.
 
   (* Lift from PURE *)
 
-  Instance hlift : PureSpec Wᴳ Word liftᵂ.
+  Instance hlift : PureSpec W Word liftᵂ.
   Proof.
     constructor.
     intros A w f.
@@ -115,8 +116,9 @@ Section Guarded.
   Abort.
 
   (* Same here *)
-  Context (hlift : PureSpec Wᴳ Word liftᵂ).
+  Context (hlift : PureSpec W Word liftᵂ).
 
-  Definition liftᴾ := liftᴾ (M := Mᴳ) (W := Wᴳ) hmono hreqlax hlift.
+  Definition liftᴾ :=
+    liftᴾ (M := Mᴳ) (W := W) hmono θᴳ_lax θᴳ_reqlax hlift.
 
 End Guarded.
